Let $u = \frac{2}{x^3}$. The equation becomes

$$
2 + u + \cosh(u) + \cosh(u) + \sinh^{-1}(u) + \sinh(u) + O(u^9) = 0
$$

$$
2 + u + 2\cosh(u) + \sinh^{-1}(u) + \sinh(u) + O(u^9) = 0
$$

Using the Taylor series expansions for
$\cosh(u) = 1 + \frac{u^2}{2!} + \frac{u^4}{4!} + \dots$
$\sinh(u) = u + \frac{u^3}{3!} + \frac{u^5}{5!} + \dots$
$\sinh^{-1}(u) = u - \frac{u^3}{6} + \frac{3u^5}{40} - \dots$
we get

$$
2 + u + 2\left(1 + \frac{u^2}{2!} + \frac{u^4}{4!} + \dots\right) + u - \frac{u^3}{6} + \frac{3u^5}{40} - \dots + u + \frac{u^3}{3!} + \frac{u^5}{5!} + \dots + O(u^9) = 0
$$

$$
2 + u + 2 + u^2 + \frac{u^4}{12} + \dots + u - \frac{u^3}{6} + \frac{3u^5}{40} - \dots + u + \frac{u^3}{6} + \frac{u^5}{120} + \dots + O(u^9) = 0
$$

$$
4 + 3u + u^2 + \frac{u^4}{12} + \frac{3u^5}{40} + \frac{u^5}{120} + \dots + O(u^9) = 0
$$

$$
4 + 3u + u^2 + \frac{u^4}{12} + \frac{10u^5}{120} + \dots + O(u^9) = 0
$$

$$
4 + 3u + u^2 + \frac{u^4}{12} + \frac{u^5}{12} + \dots + O(u^9) = 0
$$

Substituting $u = \frac{2}{x^3}$ back, we have

$$
4 + 3\left(\frac{2}{x^3}\right) + \left(\frac{2}{x^3}\right)^2 + \frac{1}{12}\left(\frac{2}{x^3}\right)^4 + \frac{1}{12}\left(\frac{2}{x^3}\right)^5 + \dots = 0
$$


$$
4 + \frac{6}{x^3} + \frac{4}{x^6} + \frac{16}{12x^{12}} + \frac{32}{12x^{15}} + \dots = 0
$$


$$
4 + \frac{6}{x^3} + \frac{4}{x^6} + \frac{4}{3x^{12}} + \frac{8}{3x^{15}} + \dots = 0
$$

Let's consider the first two terms:

$$
4 + \frac{6}{x^3} = 0
$$

$$
\frac{6}{x^3} = -4
$$

$$
x^3 = -\frac{6}{4} = -\frac{3}{2}
$$

$x = \sqrt{-\frac{3}{2}} = -\sqrt{\frac{3}{2}} \approx -1.1447$
Now let's consider the first three terms:

$$
4 + \frac{6}{x^3} + \frac{4}{x^6} = 0
$$

Let $y = \frac{1}{x^3}$. Then $4 + 6y + 4y^2 = 0$.
$4y^2 + 6y + 4 = 0$
$2y^2 + 3y + 2 = 0$
$y = \frac{-3 \pm \sqrt{9 - 4(2)(2)}}{4} = \frac{-3 \pm \sqrt{9 - 16}}{4} = \frac{-3 \pm \sqrt{-7}}{4} = \frac{-3 \pm i\sqrt{7}}{4}$
$x^3 = \frac{1}{y} = \frac{4}{-3 \pm i\sqrt{7}} = \frac{4(-3 \mp i\sqrt{7})}{(-3)^2 + (\sqrt{7})^2} = \frac{4(-3 \mp i\sqrt{7})}{9 + 7} = \frac{4(-3 \mp i\sqrt{7})}{16} = \frac{-3 \mp i\sqrt{7}}{4}$
Then $x = \sqrt{\frac{-3 \mp i\sqrt{7}}{4}}$.

Final Answer: The final answer is $\boxed{no solution}$
