Let $u = \frac{2}{x^3}$. Then the equation becomes

$$
2 + u + \cosh(u) + \cosh(u) + e^u + e^u + O(u^9) = 0
$$

$$
2 + u + 2\cosh(u) + 2e^u + O(u^9) = 0
$$

We know that $\cosh(u) = \frac{e^u + e^{-u}}{2}$, so the equation becomes

$$
2 + u + 2\left(\frac{e^u + e^{-u}}{2}\right) + 2e^u + O(u^9) = 0
$$

$$
2 + u + e^u + e^{-u} + 2e^u + O(u^9) = 0
$$

$$
2 + u + 3e^u + e^{-u} + O(u^9) = 0
$$

Using the Taylor series expansion for $e^u$,
$e^u = 1 + u + \frac{u^2}{2!} + \frac{u^3}{3!} + \dots$
$e^{-u} = 1 - u + \frac{u^2}{2!} - \frac{u^3}{3!} + \dots$
So the equation becomes

$$
2 + u + 3\left(1 + u + \frac{u^2}{2!} + \frac{u^3}{3!} + \dots\right) + 1 - u + \frac{u^2}{2!} - \frac{u^3}{3!} + \dots + O(u^9) = 0
$$

$$
2 + u + 3 + 3u + \frac{3u^2}{2} + \frac{3u^3}{6} + \dots + 1 - u + \frac{u^2}{2} - \frac{u^3}{6} + \dots + O(u^9) = 0
$$

$$
6 + 3u + 2u^2 + \frac{u^3}{3} + \dots + O(u^9) = 0
$$

Substituting $u = \frac{2}{x^3}$ back, we have

$$
6 + 3\left(\frac{2}{x^3}\right) + 2\left(\frac{2}{x^3}\right)^2 + \frac{1}{3}\left(\frac{2}{x^3}\right)^3 + \dots = 0
$$


$$
6 + \frac{6}{x^3} + \frac{8}{x^6} + \frac{8}{3x^9} + \dots = 0
$$

Let's consider the first two terms:

$$
6 + \frac{6}{x^3} = 0
$$

$$
\frac{6}{x^3} = -6
$$

$$
x^3 = -1
$$

$x = -1$
Now let's consider the first three terms:

$$
6 + \frac{6}{x^3} + \frac{8}{x^6} = 0
$$

Let $y = \frac{1}{x^3}$. Then $6 + 6y + 8y^2 = 0$.
$8y^2 + 6y + 6 = 0$
$4y^2 + 3y + 3 = 0$
$y = \frac{-3 \pm \sqrt{9 - 4(4)(3)}}{8} = \frac{-3 \pm \sqrt{9 - 48}}{8} = \frac{-3 \pm \sqrt{-39}}{8} = \frac{-3 \pm i\sqrt{39}}{8}$
$x^3 = \frac{1}{y} = \frac{8}{-3 \pm i\sqrt{39}} = \frac{8(-3 \mp i\sqrt{39})}{(-3)^2 + (\sqrt{39})^2} = \frac{8(-3 \mp i\sqrt{39})}{9 + 39} = \frac{8(-3 \mp i\sqrt{39})}{48} = \frac{-3 \mp i\sqrt{39}}{6}$
Then $x = \sqrt{\frac{-3 \mp i\sqrt{39}}{6}}$.

Final Answer: The final answer is $\boxed{no solution}$
