Let the given equation be
$$6+7+\cosh(2)+\tanh(6) = 0$$
We have $6+7=13$.
$$\cosh(x) = \frac{e^x + e^{-x}}{2}$$
$$\tanh(x) = \frac{\sinh(x)}{\cosh(x)} = \frac{e^x - e^{-x}}{e^x + e^{-x}}$$
Then
$$ \cosh(2) = \frac{e^2 + e^{-2}}{2} \approx \frac{7.389 + 0.135}{2} \approx \frac{7.524}{2} \approx 3.762$$
$$ \tanh(6) = \frac{e^6 - e^{-6}}{e^6 + e^{-6}} = \frac{403.428 - 0.002}{403.428 + 0.002} \approx \frac{403.426}{403.430} \approx 0.99999$$
The given equation can be written as
$$13+\cosh(2)+\tanh(6) = 0$$
Substitute the approximate values for $\cosh(2)$ and $\tanh(6)$:
$$13+3.762+0.99999 = 0$$
$$17.76199 \approx 0$$
The left hand side is clearly not equal to 0.
We have $\cosh(2) \approx 3.762195691$
$\tanh(6) \approx 0.9999877116$
$13 + \cosh(2) + \tanh(6) \approx 13 + 3.762195691 + 0.9999877116 \approx 17.7621834026$
The equation $6+7+\cosh(2)+\tanh(6)=0$ is false.

Final Answer: The final answer is $\boxed{False}$
