We are given the equation:

$$
6+7+\cosh(2)+\exp(6)=7
$$

First, we simplify the equation:

$$
13+\cosh(2)+\exp(6)=7
$$

We want to evaluate the expression $\cosh(2)$ and $\exp(6)$.

$$
\cosh(x) = \frac{e^x+e^{-x}}{2}
$$

$$
\cosh(2) = \frac{e^2+e^{-2}}{2} \approx \frac{7.389+0.135}{2} \approx \frac{7.524}{2} \approx 3.762
$$

$$
\exp(6) = e^6 \approx 403.42879
$$

Substituting these values into the equation, we get:

$$
13+3.762+403.42879 = 7
$$

$$
420.19079 = 7
$$

Since $420.19079 \ne 7$, the equation is false.

More precisely:
$\cosh(2) = \frac{e^2 + e^{-2}}{2} \approx 3.76219569108$
$e^6 \approx 403.428793493$
$13+\cosh(2)+e^6 \approx 13 + 3.76219569108 + 403.428793493 \approx 420.19098918408$
Thus $13+\cosh(2)+e^6=7$ is false.

Final Answer: The final answer is $\boxed{False}$
